Leanbin/Data/Vector.lean
@@ -140,7 +140,7 @@ theorem map_cons (f : α → β) (a : α) : ∀ v : Vector α n, map f (cons a v
 
 #print Vector.map₂ /-
 def map₂ (f : α → β → φ) : Vector α n → Vector β n → Vector φ n
-  | ⟨x, _⟩, ⟨y, _⟩ => ⟨List.map₂ f x y, by simp [*]⟩
+  | ⟨x, _⟩, ⟨y, _⟩ => ⟨List.zipWith f x y, by simp [*]⟩
 #align vector.map₂ Vector.map₂
 -/
 
